Update code action code

LeanCodePrompts/CodeAction.lean
@@ -1,153 +1,37 @@
 import Lean
 import LeanCodePrompts.Translate
+import Std.CodeAction.Misc
 
-open Lean Server Lsp RequestM
+open Lean Std Parser CodeAction Elab Command Server Lsp RequestM Snapshots
 
-partial def String.Iterator.findFirst? : String.Iterator → String → Option String.Pos
-  | i, pre => if i.hasNext then
-    if i.remainingToString.startsWith pre then 
-      some i.pos 
-    else 
-      i.next.findFirst? pre
-  else none
+syntax (name := translationComment) "//-" commentBody : command
 
-def String.Range.expand : String.Range → Nat → String.Range
-  | ⟨start, stop⟩, i => ⟨start - ⟨i⟩, stop + ⟨i⟩⟩
+@[command_elab translationComment]
+def translationCommentElab : CommandElab := fun _ ↦ pure ()
 
-/-- Finds the comment or doc-string in the source nearest to the given position. -/
-partial def nearestComment? (source : String) 
-  (pos : String.Pos) (start : String.Pos := ⟨0⟩) : Option String.Range := do
-    guard $ start ≤ pos
-    let firstCommentRange ← findFirstComment? source start
-    if (firstCommentRange.expand 2).contains pos then
-      some firstCommentRange
-    else
-      nearestComment? source pos (source.next firstCommentRange.stop)
-  where findFirstComment? (source : String) (init : String.Pos) : Option String.Range := do
-    let start ← (String.Iterator.mk source init).findFirst? "/-"
-    let stop ← (String.Iterator.mk source start).findFirst? "-/"
-    return ⟨start, stop + ⟨2⟩⟩
+def extractTranslationCommentBody : TSyntax ``translationComment → String
+  | ⟨.node _ _ #[_, .atom _ doc]⟩ => doc.dropRight 2
+  | stx => panic! s!"Ill-formed translation comment syntax: {stx}."
 
-/-- Extracts the text contained in a comment. -/
-def extractCommentText (comment : String) : Option String := do
-  guard $ comment.startsWith "/-"
-  guard $ comment.endsWith "-/"
-  let text := comment |>.drop 2 |>.dropRight 2
-  let c := text.front
-  if c.isAlphanum || c.isWhitespace then
-    return text
-  else
-    return text.drop 1
-
-/-
-open Parser.Command in
-def Syntax.extractComment : Syntax → Option String
-  | `($doc:docComment ) => getDocStringText doc
-  | _ => none
-
-#check getDocStringText
--/
-
-/-- A code action for translating doc-strings to Lean code using OpenAI Codex -/
-@[code_action_provider] def formaliseDocStr : CodeActionProvider := fun params snap => do
+@[command_code_action translationComment]
+def translationCommentCodeAction : CommandCodeAction := fun _params _snap _ctx _info ↦ do
+  let .node (.ofCommandInfo cmdInfo) _ := _info | return #[]
   let doc ← readDoc
-  let text := doc.meta.text
-  let source := text.source
-
-  -- the current position in the text document
-  let lspPos : Lsp.Position := params.range.end
-  -- The position from which to start searching for a comment (by default, five lines above the given position)
-  let lspBeginPos : Lsp.Position := ⟨lspPos.line - 5, 0⟩
-  let pos : String.Pos := text.lspPosToUtf8Pos lspPos
-  let beginPos : String.Pos := text.lspPosToUtf8Pos lspBeginPos
-  let comment? := nearestComment? source pos beginPos
-
-  let edit : IO TextEdit := do
-    let some ⟨start, stop⟩ := comment? | throw $ IO.userError "No input found."
-    return {
-    range := ⟨text.leanPosToLspPos <| text.toPosition start, text.leanPosToLspPos <| text.toPosition stop⟩
-    newText := ← do
-      -- the smallest node of the `InfoTree` containing the current position
-      -- let info? := snap.infoTree.findInfo? (·.contains pos)
-      -- the `Syntax` corresponding to the `Info` node
-      -- let stx? := (·.stx) <$> info?
-
-      -- the statement to be translated to Lean code
-      let stmt? : Option String := 
-        (none /- TODO: First attempt to parse using `Syntax` -/)  <|>
-        ( /- Parse as a string -/
-          let comment := source.extract start stop
-          extractCommentText comment
-        )
-
-      let translation' := snap.runTermElabM doc.meta <| translateViewM stmt?.get!
-      let translation ← EIO.toIO (λ _ => IO.userError "Translation failed.") translation'
-      return formatAsTheorem stmt? translation
-  }
-
-  let ca : CodeAction := { 
-    title := "Translate theorem docstring to Lean code", 
-    kind? := "quickfix", 
-    disabled? := 
-      match comment? with
-        | .some _ => none
-        | .none => some ⟨"No nearby comments available."⟩ }
-  return #[{ eager := ca, lazy? := some $ return {ca with 
-  edit? := some <|
-    WorkspaceEdit.ofTextEdit params.textDocument.uri <| ← edit
-    } }]
-where
-  formatAsTheorem : Option String → String → String
-    | some comment, type => s!"/-{comment}-/\nexample : {type.trim} := by sorry"
-    |     none    , type => s!"\nexample : {type.trim} := by sorry"
-
--- @[code_action_provider] def informaliseThm : CodeActionProvider := fun params snap => do
---   let doc ← readDoc
---   let text := doc.meta.text
---   let source := text.source
-
---   let edit : IO TextEdit := do
---     -- the current position in the text document
---     let pos : String.Pos := text.lspPosToUtf8Pos params.range.end
---     return {
---     range := params.range
---     newText := ← do
---       -- the smallest node of the `InfoTree` containing the current position
---       let info? := snap.infoTree.findInfo? (·.contains pos)
---       -- the `Syntax` corresponding to the `Info` node
---       let stx? := (·.stx) <$> info?
-
---       -- the statement to be translated to Lean code
---       let thm? : Option String := stx? >>= Syntax.reprint
-
---       let translation' := snap.runTermElabM doc.meta <| statementToDoc thm?.get!
---       let translation ← EIO.toIO (λ _ => IO.userError "Translation failed.") translation'
---       return "/--" ++ translation ++ "-/\n"
---   }
-
---   let ca : CodeAction := { title := "Add a docstring to a Lean theorem", kind? := "quickfix" }
---   return #[{ eager := ca, lazy? := some $ return {ca with edit? := WorkspaceEdit.ofTextEdit params.textDocument.uri $ ← edit} }]
-
--- open RequestM in
--- @[code_action_provider]
--- def readFile : CodeActionProvider := fun params _snap => do
---   let doc ← readDoc
---   let text := doc.meta.text
---   let source := text.source
---   let pos := text.lspPosToUtf8Pos params.range.end
---   let edit : TextEdit := {
---     range := params.range
---     newText :=
---       let tail := Substring.mk source pos source.endPos
---       let tail := tail.toString.splitOn "/-" |>.head!
---       "/- " ++ tail ++ "-/"
---   }
---   let ca : CodeAction := {title := "tail of source", kind? := "quickfix"}
---   return #[{eager := ca, lazy? := some $ return { ca with edit? := WorkspaceEdit.ofTextEdit params.textDocument.uri edit}}]
   
-/- 
-
-example : 1 = 1 := by
-  simp
--/
-
+  let eager := {
+    title := "Auto-formalise to Lean."
+    kind? := "quickfix",
+    isPreferred? := true }
+  return #[{
+    eager
+    lazy? := some do
+      let stx := cmdInfo.stx
+      let .some range := stx.getRange? | return eager
+      let text := extractTranslationCommentBody ⟨stx⟩
+      let res ← EIO.toIO (fun _ ↦ .userError "Translation failed.") <| _snap.runTermElabM doc.meta <|
+          translateViewM text
+      return { eager with
+        edit? := some <| .ofTextEdit doc.meta.uri {
+          range := doc.meta.text.utf8RangeToLspRange range,
+          newText := s!"/-- {text}-/\n{res}"}}
+    }]
